src/coq/Theory/TopLevelRefinements.v
@@ -158,6 +158,25 @@ Module Type TopLevelRefinements (IS : InterpreterStack) (TOP : LLVMTopLevel IS).
       apply eutt_tt_to_eq_prod, eutt_interp_state; auto.
     Qed.
 
+    Lemma refine_01_eq : forall (t1 t2 : itree L0 dvalue) (g : global_env),
+        eutt eq t1 t2 -> eutt eq (interp_global t1 g) (interp_global t2 g).
+    Proof using.
+      intros t1 t2 g REF.
+      rewrite eutt_subrel;
+        [ reflexivity | apply prod_rel_eq | ].
+      eapply eutt_interp_state; eauto.
+    Qed.
+
+    (* No stack *)
+    Lemma refine_01_cfg_eq : forall (t1 t2 : itree instr_E dvalue) (g : global_env),
+        eutt eq t1 t2 -> eutt eq (interp_global t1 g) (interp_global t2 g).
+    Proof using.
+      intros t1 t2 g REF.
+      rewrite eutt_subrel;
+        [ reflexivity | apply prod_rel_eq | ].
+      eapply eutt_interp_state; eauto.
+    Qed.
+
     Lemma refine_12 : forall t1 t2 l,
         refine_L1 t1 t2 -> refine_L2 (interp_local_stack t1 l) (interp_local_stack t2 l).
     Proof using.
@@ -165,10 +184,30 @@ Module Type TopLevelRefinements (IS : InterpreterStack) (TOP : LLVMTopLevel IS).
       apply eutt_tt_to_eq_prod, eutt_interp_state; auto.
     Qed.
 
+    Lemma refine_12_eq : forall (t1 t2 : itree L1 res_L1) (l : local_env * stack),
+        eutt eq t1 t2 ->  eutt eq (interp_local_stack t1 l) (interp_local_stack t2 l).
+    Proof using.
+      intros * REF.
+      rewrite eutt_subrel;
+        [ reflexivity | apply prod_rel_eq | ].
+      eapply eutt_interp_state; eauto.
+    Qed.
+
+    (* No stack, used for interp_cfg instead of interp_mcfg *)
+    (* TODO: Generalize itree event type? *)
+    Lemma refine_12_cfg_eq : forall (t1 t2 : itree (CallE +' IntrinsicE +' LLVMEnvE +' MemoryE +' PickUvalueE +' OOME +' UBE +' DebugE +' FailureE) res_L1) (l : local_env),
+        eutt eq t1 t2 ->  eutt eq (interp_local t1 l) (interp_local t2 l).
+    Proof using.
+      intros * REF.
+      rewrite eutt_subrel;
+        [ reflexivity | apply prod_rel_eq | ].
+      eapply eutt_interp_state; eauto.
+    Qed.
+
     Lemma refine_23 : forall t1 t2 sid m,
         refine_L2 t1 t2 -> refine_L3 (interp_memory_spec refine_res2 t1 sid m) (interp_memory_spec refine_res2 t2 sid m).
     Proof using.
-      intros t1 t2 sid ms REF t Ht.
+      intros * REF t Ht.
       exists t; split.
       - unfold L3 in *.
         unfold refine_L2 in *.
@@ -177,9 +216,37 @@ Module Type TopLevelRefinements (IS : InterpreterStack) (TOP : LLVMTopLevel IS).
       - reflexivity.
     Qed.
 
+    Lemma refine_23_eq :
+      forall (t1 t2 : itree L2 (local_env * stack * res_L1)) (sid : StoreId.store_id) (m : MemState),
+        eutt eq t1 t2 ->
+        refine_L3_eq (interp_memory_spec eq t1 sid m) (interp_memory_spec eq t2 sid m).
+    Proof using.
+      intros * REF t Ht.
+      exists t; split.
+      - unfold L3 in *.
+        unfold refine_L2 in *.
+        eapply interp_memory_prop_Proper_eq in Ht; try typeclasses eauto; eauto.
+      - reflexivity.
+    Qed.
+
     (* Things are different for L4 and L5: we get into the [Prop] monad. *)
     Lemma refine_34 : forall t1 t2,
         refine_L3 t1 t2 -> refine_L4 (model_undef refine_res3 t1) (model_undef refine_res3 t2).
+    Proof using.
+      intros t1 t2 REF t Ht.
+      exists t; split.
+      - unfold model_undef in *.
+        unfold refine_L3 in *.
+        destruct Ht as [t_pre [T2 MODEL]].
+        specialize (REF _ T2).
+        destruct REF as [t_pre1 [T1 EUTT]].
+        exists t_pre1; split; auto.
+        eapply interp_prop_oom_Proper_eq in MODEL; try typeclasses eauto; eauto.
+      - reflexivity.
+    Qed.
+
+    Lemma refine_34_eq : forall t1 t2,
+        refine_L3_eq t1 t2 -> refine_L4_eq (model_undef eq t1) (model_undef eq t2).
     Proof using.
       intros t1 t2 REF t Ht.
       exists t; split.
@@ -209,6 +276,22 @@ Module Type TopLevelRefinements (IS : InterpreterStack) (TOP : LLVMTopLevel IS).
         rewrite EQ; auto.
     Qed.
 
+    Lemma refine_45_eq : forall Pt1 Pt2,
+        refine_L4_eq Pt1 Pt2 -> refine_L5_eq (model_UB Pt1) (model_UB Pt2).
+    Proof using.
+      intros Pt1 Pt2 HR t2 HM.
+      destruct HM as [Pt2_t2 | [ub [Pt2_ub UB]]].
+      - specialize (HR t2 Pt2_t2) as [t1 [Pt1_t1 EQ]].
+        exists t1.
+        split; auto.
+        left; auto.
+      - specialize (HR ub Pt2_ub) as [ub1 [Pt1_ub1 EQ]].
+        exists t2.
+        split; try reflexivity.
+        right. exists ub1; split; auto.
+        rewrite EQ; auto.
+    Qed.
+
     Lemma refine_56 : forall Pt1 Pt2,
         refine_L5 Pt1 Pt2 -> refine_L6 Pt1 Pt2.
     Proof using.
@@ -219,7 +302,18 @@ Module Type TopLevelRefinements (IS : InterpreterStack) (TOP : LLVMTopLevel IS).
         typeclasses eauto.
     Qed.
 
+    Lemma refine_56_eq : forall Pt1 Pt2,
+        refine_L5_eq Pt1 Pt2 -> refine_L6_eq Pt1 Pt2.
+    Proof using.
+      intros Pt1 Pt2 HR t2 HM.
+      apply HR in HM as (t1 & HPt1 & HPT1).
+        exists t1; split; auto;
+        apply eutt_refine_oom_h; auto.
+        typeclasses eauto.
+    Qed.
+
     Hint Resolve refine_12 refine_23 refine_34 refine_45 refine_56 : refine_xx.
+    Hint Resolve refine_12_eq refine_23_eq refine_34_eq refine_45_eq refine_56_eq : refine_xx.
 
     Variable ret_typ : dtyp.
     Variable entry : string.
